examples modification complete

increment/IncrementA.v
@@ -2,22 +2,22 @@ Require Import CRIS.
 Require Import ImpPrelude.
 Require Import SchHeader SchA SchTactics.
 Require Import MemHeader MemA.
-Require Import IncrementHeader.
+From CRIS.increment Require Import Header.
 
 Module IncrementA. Section IncrementA.
   Context `{_sinvG: !sinvG Γ Σ α β τ _I _S}.
   Context `{_memG: !memG}.
   Context `{_schG: !schG}.
                      
-  Definition increment_spec u : fspec :=
-    sch_fspec u
+  Definition increment_spec : fspec :=
+    fspec_sch ∅
       (fspec_simple (λ bofs,
         ((λ varg, ⌜varg = [Vptr bofs]↑⌝),
         (λ vret, True))
       ))%I.
 
-  Definition sp u : alist string fspec :=
-    [(IncrementHdr.increment, increment_spec u)].
+  Definition sp : alist string fspec :=
+    [(IncrementHdr.increment, increment_spec)].
 
   Definition scopes : list string := [].
 
@@ -38,16 +38,16 @@ Module IncrementA. Section IncrementA.
   Definition increment : list val → itree hmodE val :=
     λ arg, increment2 arg.
 
-  Definition fnsems u :=
-    [(IncrementHdr.increment, (wmask_all, scopes, mk_specbody (increment_spec u) (cfunN increment)))].
+  Definition fnsems :=
+    [(IncrementHdr.increment, (wmask_all, scopes, mk_specbody (increment_spec) (cfunN increment)))].
 
-  Program Definition Mod u : SMod.t := {|
+  Program Definition Mod : SMod.t := {|
     SMod.scopes := scopes;
-    SMod.fnsems := fnsems u;
+    SMod.fnsems := fnsems;
     SMod.initial_st := [];
   |}.
   Solve All Obligations with prove_scope.
   Next Obligation. prove_nodup. Qed.
 
-  Definition t u sp : HMod.t := Seal.sealing CRIS (SMod.to_hmod sp (Mod u)).
+  Definition t : HMod.t := Seal.sealing CRIS (SMod.to_hmod (to_sp (SchAS.sp ∅ sp_empty)) Mod).
 End IncrementA. End IncrementA.
