spinlock/SpinLockMainHeader.v
@@ -1,6 +1,0 @@
-Require Import Common.
-
-Module SpinLockMainHdr.
-  Definition main := "CRIS_init".
-  Definition incr := "incr".
-End SpinLockMainHdr.
