cannon/CannonAll.v
@@ -8,8 +8,8 @@ Module CannonAll.
   Import inv_instances.
   Local Instance Γ : HRA := ##[invΓ; cannonΓ].
   Local Instance Σ : GRA := ##[Γ; invΣ].
-  Local Definition irΓ : Γ := **[ir_invΓ 1; CannonAS.irΓ].
-  Local Definition irΣ : Σ := **[irΓ; ir_invΣ 1].
+  Local Definition irΓ : Γ := **[ir_invΓ; CannonAS.irΓ].
+  Local Definition irΣ : Σ := **[irΓ; ir_invΣ].
 
   Local Lemma irΣ_valid : ✓ (irΣ ⋅ initial_resource_own_admin).
   Proof.
@@ -78,8 +78,7 @@ Module CannonAll.
     destruct (H (irΣ ⋅ initial_resource_own_admin)).
     { apply irΣ_valid. }
     { clear H. simplify_res.
-      {
-        iPoseProof (CannonAS.ReadyBall with "[H12]") as "[R B]"; eauto.
+      { iPoseProof (CannonAS.ReadyBall with "[H12]") as "[R B]"; eauto.
         iSplitL "R".
         { iFrame. }
         unfold_pre_post. iFrame. eauto.
