increment/IncrementIAproof.v
@@ -1,7 +1,7 @@
 Require Import CRIS.
 Require Import SchHeader SchA SchTactics.
 Require Import ImpPrelude MemHeader MemA.
-Require Import IncrementHeader IncrementI IncrementA.
+From CRIS.increment Require Import Header IncrementI IncrementA.
 
 Module IncrementIA. Section IncrementIA.
   Context `{_sinvG: !sinvG Γ Σ α β τ _I _S}.
@@ -10,21 +10,21 @@ Module IncrementIA. Section IncrementIA.
 
   Definition Ist : nat → alist key Any.t → alist key Any.t → iProp Σ := λ _ _ _, emp%I.
 
-  Context (u_s : univ_id).
-  Context (sp_s sp_user_s sp_mem : string → option fspec).
+  Context (sp_mem : string → option fspec).
 
-  Context (SchInSpS : sp_incl (SchAS.sp u_s sp_user_s) sp_s).
+  Local Lemma SchInSpS : sp_incl (SchAS.sp ∅ sp_empty) (to_sp (SchAS.sp ∅ sp_empty)).
+  Proof. split; ss. rewrite /SchAS.sp; unseal CRIS; s; prove_nodup. Qed. 
 
   Local Definition MemA := (MemA.t sp_mem).
-  Local Definition IncrementA := (IncrementA.t u_s sp_s).
+  Local Definition IncrementA := (IncrementA.t).
   Local Definition IncrementI := (IncrementI.t).
   Local Definition IstFull := (IstProd (IstSB IncrementA.(HMod.scopes) Ist) IstEq).
   Local Definition MA := (IncrementA ★ MemA).
   Local Definition MI := (IncrementI ★ MemA).
 
   Lemma increment_simF : HSim.sim_fun open MA MI IstFull IncrementHdr.increment.
-  Proof using SchInSpS.
-    init_simF u_s 0.
+  Proof using.
+    init_simF.
     steps_l. iDestruct "ASM" as "[TID [-> ->]]".
     destruct q2 as [blk ofs]. rename q1 into tid. hss.
     steps_l.
@@ -32,10 +32,10 @@ Module IncrementIA. Section IncrementIA.
       rewrite /IncrementA.increment2.
       steps_l. steps_r.
 
-      sch_yield_r. iFrame "IST TID".
+      sch_yield_r; first apply SchInSpS. iFrame "IST TID".
       clear dependent nths st_src st_tgt; iIntros (nths st_s st_t _ _) "IST TID". steps_r.
 
-      sch_yield_r. iFrame "IST TID".
+      sch_yield_r; first apply SchInSpS. iFrame "IST TID".
       clear nths st_s st_t; iIntros (nths st_s st_t _ _) "IST TID". steps_r. sch_yield_l.
 
       iApply wsim_reset.
@@ -46,7 +46,7 @@ Module IncrementIA. Section IncrementIA.
       unfold_iter_l. unfold_iter_r.
       steps_l. steps_r.
 
-      sch_yield_r. iFrame "IST TID".
+      sch_yield_r; first apply SchInSpS. iFrame "IST TID".
       clear nths st_s st_t; iIntros (nths st_s st_t _ _) "IST TID". sch_yield_l.
 
       steps_l.
@@ -55,9 +55,9 @@ Module IncrementIA. Section IncrementIA.
 
       force_l false; steps_l. forces_l. iFrame "PT". steps_l. sch_yield_l. steps_l.
       unfold_iter_l. steps_l.
-      sch_yield_r. iFrame "IST TID".
+      sch_yield_r; first apply SchInSpS. iFrame "IST TID".
       clear nths st_s st_t; iIntros (nths st_s st_t _ _) "IST TID".
-      sch_yield_r. iFrame "IST TID".
+      sch_yield_r; first apply SchInSpS. iFrame "IST TID".
       clear nths st_s st_t; iIntros (nths st_s st_t _ _) "IST TID".
 
       (* We are getting memory resource for cas here *)
@@ -70,9 +70,9 @@ Module IncrementIA. Section IncrementIA.
         iSplitL "". { repeat (iSplitL; et). s. des_ifs. }
         steps_r. iDestruct "GRT" as "[[% [PT _]] %]". hss_r. steps_r. des_ifs.
         force_l true. steps_l. forces_l. iFrame "PT". steps_l.
-        sch_yield_r. iFrame "IST TID".
+        sch_yield_r; first apply SchInSpS. iFrame "IST TID".
         clear nths st_s st_t; iIntros (nths st_s st_t _ _) "IST TID". steps_r.
-        sch_yield_r. iFrame "IST TID".
+        sch_yield_r; first apply SchInSpS. iFrame "IST TID".
         clear nths st_s st_t; iIntros (nths st_s st_t _ _) "IST TID".
         rewrite _EQ. steps_r.
 
@@ -84,9 +84,9 @@ Module IncrementIA. Section IncrementIA.
         { repeat iSplitL; et. s. des_ifs. }
         steps_r. iDestruct "GRT" as "[[% [PT _]] %]". hss_r. steps_r. des_ifs.
         force_l false; steps_l. force_l; iFrame "PT". steps_l.
-        sch_yield_r. iFrame "IST TID".
+        sch_yield_r; first apply SchInSpS. iFrame "IST TID".
         clear nths st_s st_t; iIntros (nths st_s st_t _ _) "IST TID". steps_r.
-        sch_yield_r. iFrame "IST TID".
+        sch_yield_r; first apply SchInSpS. iFrame "IST TID".
         clear nths st_s st_t; iIntros (nths st_s st_t _ _) "IST TID".
         rewrite _EQ. steps_r. sch_yield_l. steps_l.
         by_coind "CIH". iFrame.
